module plfa.Naturals where

data ℕ : Set where
  zero : ℕ
  suc  : ℕ → ℕ


{-# BUILTIN NATURAL ℕ #-}

import Relation.Binary.PropositionalEquality as Eq
open Eq using (_≡_; refl)
open Eq.≡-Reasoning using (begin_; _≡⟨⟩_; _∎)


_+_ : ℕ → ℕ → ℕ
zero + n = n
(suc m) + n = suc (m + n)


_ : 2 + 3 ≡ 5
_ =
  begin
    2 + 3
  ≡⟨⟩
    suc (1 + 3)
  ≡⟨⟩
    suc (suc (0 + 3))
  ≡⟨⟩
    suc (suc 3)
  ≡⟨⟩
    5
  ∎

_ : 2 + 3 ≡ 5
_ = refl


{- Exercise +-example -}
_ : 3 + 4 ≡ 7
_ =
  begin
    3 + 4
  ≡⟨⟩
    suc (2 + 4)
  ≡⟨⟩
    suc (suc (1 + 4))
  ≡⟨⟩
    suc (suc (suc (0 + 4)))
  ≡⟨⟩
    suc (suc (suc 4))
  ≡⟨⟩
    7
  ∎
